dist/gcc-compatible/Hacl_RSAPSS.h
@@ -35,8 +35,8 @@ extern "C" {
 #include "krml/internal/target.h"
 
 
+#include "Hacl_Streaming_SHA2.h"
 #include "Hacl_Spec.h"
-#include "Hacl_Hash_SHA2.h"
 #include "Hacl_Bignum_Base.h"
 
 /**
