specs/lemmas/Spec.SHA2.Lemmas.fsti
@@ -9,6 +9,11 @@ val update_224_256: hash:words_state SHA2_256 ->
   Lemma
     (ensures (Spec.SHA2.(update SHA2_256 hash block == update SHA2_224 hash block)))
 
+val update_224_256': st:words_state SHA2_256 ->
+  block:bytes{Seq.length block = block_length SHA2_256} ->
+  Lemma
+    (ensures (Spec.Agile.Hash.(update SHA2_256 st block == update SHA2_224 st block)))
+
 val update_multi_224_256: hash:words_state SHA2_256 -> blocks:bytes_blocks SHA2_256 ->
   Lemma
     (ensures (Spec.Agile.Hash.update_multi SHA2_256 hash () blocks ==
